crates/algorithms/sha3/proofs/fstar/extraction/Libcrux_sha3.Neon.fst
@@ -3,12 +3,34 @@ module Libcrux_sha3.Neon
 open FStar.Mul
 open Core_models
 
+#push-options "--fuel 0 --ifuel 1 --z3rlimit 200 --split_queries always"
+
 /// A SHA3 224 implementation.
 let sha224 (digest data: t_Slice u8)
     : Prims.Pure (t_Slice u8)
       (requires (Core_models.Slice.impl__len #u8 digest <: usize) =. mk_usize 28)
-      (fun _ -> Prims.l_True) =
+      (ensures
+        fun digest_future ->
+          let digest_future:t_Slice u8 = digest_future in
+          b2t
+          ((Core_models.Slice.impl__len #u8 digest_future <: usize) =.
+            (Core_models.Slice.impl__len #u8 digest <: usize)
+            <:
+            bool) /\
+          (digest_future <: t_Slice u8) ==
+          (Hacspec_sha3.Sponge.keccak (Core_models.Slice.impl__len #u8 digest)
+              (mk_usize 144) (mk_u8 6) data
+            <:
+            t_Slice u8)) =
   let dummy:t_Array u8 (mk_usize 28) = Rust_primitives.Hax.repeat (mk_u8 0) (mk_usize 28) in
+  let _:Prims.unit =
+    let inputs : t_Array (t_Slice u8) (mk_usize 2) =
+      let l : list (t_Slice u8) = [ data; data ] in
+      FStar.Pervasives.assert_norm (List.Tot.length l == 2);
+      Rust_primitives.Hax.array_of_list 2 l in
+    EquivImplSpec.Sponge.Arm64.Driver.lemma_keccak2_arm64
+      (mk_usize 144) (mk_u8 6) inputs digest (dummy <: t_Slice u8)
+  in
   let (tmp0: t_Slice u8), (tmp1: t_Array u8 (mk_usize 28)) =
     Libcrux_sha3.Generic_keccak.Simd128.keccak2 (mk_usize 144)
       (mk_u8 6)
@@ -27,8 +49,28 @@ let sha224 (digest data: t_Slice u8)
 let sha256 (digest data: t_Slice u8)
     : Prims.Pure (t_Slice u8)
       (requires (Core_models.Slice.impl__len #u8 digest <: usize) =. mk_usize 32)
-      (fun _ -> Prims.l_True) =
+      (ensures
+        fun digest_future ->
+          let digest_future:t_Slice u8 = digest_future in
+          b2t
+          ((Core_models.Slice.impl__len #u8 digest_future <: usize) =.
+            (Core_models.Slice.impl__len #u8 digest <: usize)
+            <:
+            bool) /\
+          (digest_future <: t_Slice u8) ==
+          (Hacspec_sha3.Sponge.keccak (Core_models.Slice.impl__len #u8 digest)
+              (mk_usize 136) (mk_u8 6) data
+            <:
+            t_Slice u8)) =
   let dummy:t_Array u8 (mk_usize 32) = Rust_primitives.Hax.repeat (mk_u8 0) (mk_usize 32) in
+  let _:Prims.unit =
+    let inputs : t_Array (t_Slice u8) (mk_usize 2) =
+      let l : list (t_Slice u8) = [ data; data ] in
+      FStar.Pervasives.assert_norm (List.Tot.length l == 2);
+      Rust_primitives.Hax.array_of_list 2 l in
+    EquivImplSpec.Sponge.Arm64.Driver.lemma_keccak2_arm64
+      (mk_usize 136) (mk_u8 6) inputs digest (dummy <: t_Slice u8)
+  in
   let (tmp0: t_Slice u8), (tmp1: t_Array u8 (mk_usize 32)) =
     Libcrux_sha3.Generic_keccak.Simd128.keccak2 (mk_usize 136)
       (mk_u8 6)
@@ -47,8 +89,28 @@ let sha256 (digest data: t_Slice u8)
 let sha384 (digest data: t_Slice u8)
     : Prims.Pure (t_Slice u8)
       (requires (Core_models.Slice.impl__len #u8 digest <: usize) =. mk_usize 48)
-      (fun _ -> Prims.l_True) =
+      (ensures
+        fun digest_future ->
+          let digest_future:t_Slice u8 = digest_future in
+          b2t
+          ((Core_models.Slice.impl__len #u8 digest_future <: usize) =.
+            (Core_models.Slice.impl__len #u8 digest <: usize)
+            <:
+            bool) /\
+          (digest_future <: t_Slice u8) ==
+          (Hacspec_sha3.Sponge.keccak (Core_models.Slice.impl__len #u8 digest)
+              (mk_usize 104) (mk_u8 6) data
+            <:
+            t_Slice u8)) =
   let dummy:t_Array u8 (mk_usize 48) = Rust_primitives.Hax.repeat (mk_u8 0) (mk_usize 48) in
+  let _:Prims.unit =
+    let inputs : t_Array (t_Slice u8) (mk_usize 2) =
+      let l : list (t_Slice u8) = [ data; data ] in
+      FStar.Pervasives.assert_norm (List.Tot.length l == 2);
+      Rust_primitives.Hax.array_of_list 2 l in
+    EquivImplSpec.Sponge.Arm64.Driver.lemma_keccak2_arm64
+      (mk_usize 104) (mk_u8 6) inputs digest (dummy <: t_Slice u8)
+  in
   let (tmp0: t_Slice u8), (tmp1: t_Array u8 (mk_usize 48)) =
     Libcrux_sha3.Generic_keccak.Simd128.keccak2 (mk_usize 104)
       (mk_u8 6)
@@ -67,8 +129,28 @@ let sha384 (digest data: t_Slice u8)
 let sha512 (digest data: t_Slice u8)
     : Prims.Pure (t_Slice u8)
       (requires (Core_models.Slice.impl__len #u8 digest <: usize) =. mk_usize 64)
-      (fun _ -> Prims.l_True) =
+      (ensures
+        fun digest_future ->
+          let digest_future:t_Slice u8 = digest_future in
+          b2t
+          ((Core_models.Slice.impl__len #u8 digest_future <: usize) =.
+            (Core_models.Slice.impl__len #u8 digest <: usize)
+            <:
+            bool) /\
+          (digest_future <: t_Slice u8) ==
+          (Hacspec_sha3.Sponge.keccak (Core_models.Slice.impl__len #u8 digest)
+              (mk_usize 72) (mk_u8 6) data
+            <:
+            t_Slice u8)) =
   let dummy:t_Array u8 (mk_usize 64) = Rust_primitives.Hax.repeat (mk_u8 0) (mk_usize 64) in
+  let _:Prims.unit =
+    let inputs : t_Array (t_Slice u8) (mk_usize 2) =
+      let l : list (t_Slice u8) = [ data; data ] in
+      FStar.Pervasives.assert_norm (List.Tot.length l == 2);
+      Rust_primitives.Hax.array_of_list 2 l in
+    EquivImplSpec.Sponge.Arm64.Driver.lemma_keccak2_arm64
+      (mk_usize 72) (mk_u8 6) inputs digest (dummy <: t_Slice u8)
+  in
   let (tmp0: t_Slice u8), (tmp1: t_Array u8 (mk_usize 64)) =
     Libcrux_sha3.Generic_keccak.Simd128.keccak2 (mk_usize 72)
       (mk_u8 6)
@@ -84,8 +166,25 @@ let sha512 (digest data: t_Slice u8)
   digest
 
 /// A SHAKE128 implementation.
-let shake128 (v_LEN: usize) (digest: t_Array u8 v_LEN) (data: t_Slice u8) : t_Array u8 v_LEN =
+let shake128 (v_LEN: usize) (digest: t_Array u8 v_LEN) (data: t_Slice u8)
+    : Prims.Pure (t_Array u8 v_LEN)
+      (requires v_LEN <. (Core_models.Num.impl_usize__MAX -! mk_usize 200 <: usize))
+      (ensures
+        fun digest_future ->
+          let digest_future:t_Array u8 v_LEN = digest_future in
+          (digest_future <: t_Array u8 v_LEN) ==
+          (Hacspec_sha3.Sponge.keccak v_LEN (mk_usize 168) (mk_u8 31) data
+            <:
+            t_Array u8 v_LEN)) =
   let dummy:t_Array u8 v_LEN = Rust_primitives.Hax.repeat (mk_u8 0) v_LEN in
+  let _:Prims.unit =
+    let inputs : t_Array (t_Slice u8) (mk_usize 2) =
+      let l : list (t_Slice u8) = [ data; data ] in
+      FStar.Pervasives.assert_norm (List.Tot.length l == 2);
+      Rust_primitives.Hax.array_of_list 2 l in
+    EquivImplSpec.Sponge.Arm64.Driver.lemma_keccak2_arm64
+      (mk_usize 168) (mk_u8 31) inputs (digest <: t_Slice u8) (dummy <: t_Slice u8)
+  in
   let (tmp0: t_Array u8 v_LEN), (tmp1: t_Array u8 v_LEN) =
     Libcrux_sha3.Generic_keccak.Simd128.keccak2 (mk_usize 168)
       (mk_u8 31)
@@ -101,8 +200,25 @@ let shake128 (v_LEN: usize) (digest: t_Array u8 v_LEN) (data: t_Slice u8) : t_Ar
   digest
 
 /// A SHAKE256 implementation.
-let shake256 (v_LEN: usize) (digest: t_Array u8 v_LEN) (data: t_Slice u8) : t_Array u8 v_LEN =
+let shake256 (v_LEN: usize) (digest: t_Array u8 v_LEN) (data: t_Slice u8)
+    : Prims.Pure (t_Array u8 v_LEN)
+      (requires v_LEN <. (Core_models.Num.impl_usize__MAX -! mk_usize 200 <: usize))
+      (ensures
+        fun digest_future ->
+          let digest_future:t_Array u8 v_LEN = digest_future in
+          (digest_future <: t_Array u8 v_LEN) ==
+          (Hacspec_sha3.Sponge.keccak v_LEN (mk_usize 136) (mk_u8 31) data
+            <:
+            t_Array u8 v_LEN)) =
   let dummy:t_Array u8 v_LEN = Rust_primitives.Hax.repeat (mk_u8 0) v_LEN in
+  let _:Prims.unit =
+    let inputs : t_Array (t_Slice u8) (mk_usize 2) =
+      let l : list (t_Slice u8) = [ data; data ] in
+      FStar.Pervasives.assert_norm (List.Tot.length l == 2);
+      Rust_primitives.Hax.array_of_list 2 l in
+    EquivImplSpec.Sponge.Arm64.Driver.lemma_keccak2_arm64
+      (mk_usize 136) (mk_u8 31) inputs (digest <: t_Slice u8) (dummy <: t_Slice u8)
+  in
   let (tmp0: t_Array u8 v_LEN), (tmp1: t_Array u8 v_LEN) =
     Libcrux_sha3.Generic_keccak.Simd128.keccak2 (mk_usize 136)
       (mk_u8 31)
@@ -116,3 +232,5 @@ let shake256 (v_LEN: usize) (digest: t_Array u8 v_LEN) (data: t_Slice u8) : t_Ar
   let dummy:t_Array u8 v_LEN = tmp1 in
   let _:Prims.unit = () in
   digest
+
+#pop-options
